Refactor: set theory into Logic

haskell/Shake.hs
@@ -1,0 +1,13 @@
+module  Main (main) where
+
+import Development.Shake
+import System.FilePath
+
+main :: IO ()
+main = shake shakeOptions $ do
+    want ["Test.vo"]
+
+    "*.vo" %> \out -> do
+        let src = out -<.> "v"
+        needed [src]
+        cmd "coqc" src "-Q . Logic"
