coq/set/Core/Functional.v
@@ -1,5 +1,0 @@
-Require Import Core.Set.
-Require Import Core.Equal.
-
-Definition functional (p:set -> set -> Prop) : Prop :=
-    forall (x y y':set), p x y -> p x y' -> y == y'.
