coq/set/Normal/InListOf.v
@@ -1,5 +1,0 @@
-Require Import List.
-
-Require Import Core.Set.
-
-Definition inListOf (x xs:set) : Prop := In x (toList xs).
