coq/Logic/Lang1/Apply.v
@@ -1,0 +1,68 @@
+Require Import List.
+
+Require Import Logic.Func.Replace.
+Require Import Logic.Func.Composition.
+
+Require Import Logic.Set.Set.
+Require Import Logic.Set.Equal.
+
+Require Import Logic.Lang1.Free.
+Require Import Logic.Lang1.Valid.
+Require Import Logic.Lang1.Syntax.
+Require Import Logic.Lang1.Semantics.
+Require Import Logic.Lang1.Relevance.
+Require Import Logic.Lang1.Environment.
+Require Import Logic.Lang1.Substitution.
+
+(* A formula with a free variable could be viewed as a predicate which needs to *)
+(* be 'evaluated' at some variable, where such evaluation corresponds to a      *)
+(* variable substitution. In the following, we formalize this evaluation by     *)
+(* substituting the variable '0' by the argument 'n'. This choice of variable   *)
+(* '0' is arbitrary, but having this default choice leads to simpler syntax as  *)
+(* there is no need to spell out which variable is being replaced. There is     *)
+(* nothing deep here, as we are just creating a new formula from an old one.    *)
+(* The ability to apply a formula viewed as predicate to variables is important *)
+(* for two variables, and is needed to express the axiom schema of replacement. *)
+
+Definition apply (p:Formula) (n:nat) : Formula := fmap (replace 0 n) p.
+
+(* Same idea, but with two variables.                                           *)
+Definition apply2 (p:Formula) (n m:nat) : Formula := fmap (replace2 0 1 n m) p.
+
+(* The semantics of 'apply p n' in an environement where n is bound to set x    *)
+(* is the same as the semantics of p in an environment where 0 is bound to x.   *)
+(* However, we cannot hope to obtain this semantics equivalence without         *)
+(* assuming that the replacement of variable 0 by n is a valid substitution     *)
+(* for p. Also, n cannot already be a free variable of p.                       *)
+
+Lemma evalApply1 : forall (e:Env) (p:Formula) (n:nat) (x:set),
+    Valid (replace 0 n) p ->
+    ~In n (Fr p)        ->
+    eval1 e (apply p n) n x <-> eval1 e p 0 x.
+Proof.
+    unfold eval1, apply. intros e p n x H1 H2. rewrite Substitution.
+    - apply relevance. intros m H3. apply bindReplace. intros H4. 
+      subst. apply H2. assumption. 
+    - assumption.
+Qed.
+
+
+(* The semantics of 'apply2 p n m' in an environment where n is bound to x and  *)
+(* m is bound to y, is the same as the semantics of p in an environment where 0 *)
+(* is bound to x and 1 is bound to y, with the obvious caveat.                  *)
+Lemma evalApply2 : forall (e:Env) (p:Formula) (n m:nat) (x y:set),
+    Valid (replace2 0 1 n m) p ->
+    ~In n (Fr p)  ->
+    ~In m (Fr p)  ->
+    n <> m          ->
+    eval2 e (apply2 p n m) n m x y <-> eval2 e p 0 1 x y.
+Proof.
+    unfold eval2, apply2. intros e p n m x y H1 H2 H3 H4. rewrite Substitution.
+    - apply relevance. intros r H5. unfold comp. apply bindReplace2.
+        + auto.
+        + apply H4.                                     (* <- H4 *)
+        + intros H6. apply H2. rewrite H6. assumption.  (* <- H2 *)
+        + intros H6. apply H3. rewrite H6. assumption.  (* <- H3 *)
+    - apply H1.                                         (* <- H1 *)
+Qed.
+
