coq/Logic/Lang1/Free.v
@@ -1,0 +1,30 @@
+Require Import Logic.Nat.Eq.
+Require Import Logic.Class.Eq.
+Require Import Logic.List.Remove.
+
+Require Import Logic.Lang1.Syntax.
+
+
+(* Free variables of a formula.                                                 *)
+Fixpoint Fr (p:Formula) : list nat :=
+    match p with
+    | Bot       => nil
+    | Elem n m  => cons n (cons m nil)
+    | Imp p q   => Fr p ++ Fr q
+    | All n p   => remove n (Fr p)
+    end.  
+
+(*
+Lemma free_map : forall (f:nat -> nat) (p:Formula),
+    incl (Fr (fmap f p)) (map f (Fr p)).
+Proof.
+    intros f. induction p as [|x y|p1 IH1 p2 IH2|x p1 IH1]; simpl.
+    - apply incl_refl.
+    - apply incl_refl.
+    - rewrite map_app. apply incl_app.
+        + apply incl_appl, IH1.
+        + apply incl_appr, IH2.
+    - apply incl_tran with (remove eqDec (f x) (map f (Fr p1))). 
+
+Show.
+*)
