coq/Logic/Lang1/Relevance.v
@@ -1,0 +1,70 @@
+Require Import List.
+
+Require Import Logic.Nat.Eq.
+Require Import Logic.Class.Eq.
+Require Import Logic.List.Remove.
+
+Require Import Logic.Set.Set.
+Require Import Logic.Set.Equal.
+
+Require Import Logic.Lang1.Free.
+Require Import Logic.Lang1.Syntax.
+Require Import Logic.Lang1.Semantics.
+Require Import Logic.Lang1.Environment.
+
+Definition envEqualOn (p:Formula) (e e':Env) : Prop :=
+    forall (n:nat), In n (Fr p) -> e n == e' n.
+
+Lemma relevance : forall (e e':Env) (p:Formula), 
+    envEqualOn p e e' -> eval e p <-> eval e' p.
+Proof.
+    intros e e' p. unfold envEqualOn. revert e e'.
+    induction p as [|n m|p1 IH1 p2 IH2|n p1 IH1]; intros e e' H; simpl.
+    - tauto.
+    - split. 
+        + apply elemCompatLR; apply H.
+            { left. reflexivity. }
+            { right. left. reflexivity. }
+        + apply elemCompatLR; apply equalSym; apply H.
+            { left. reflexivity. }
+            { right. left. reflexivity. }
+    - rewrite (IH1 e e'), (IH2 e e').
+        + tauto.
+        + intros n H'. apply H. simpl. apply in_or_app. right. assumption.
+        + intros n H'. apply H. simpl. apply in_or_app. left.  assumption.
+    - split; intros H' x.
+        + rewrite (IH1 (bind e' n x) (bind e n x)). 
+            { apply H'. }
+            { intros m.  destruct (eqDec n m) as [E|E].
+                { subst. rewrite bindSame, bindSame. intros. apply equalRefl. }
+                { rewrite bindDiff, bindDiff.
+                    { intros H''. apply equalSym. apply H. simpl. 
+                      apply remove_still; assumption. }
+                    { assumption. }
+                    { assumption. }}}
+        + rewrite (IH1 (bind e n x) (bind e' n x)). 
+            { apply H'. }
+            { intros m H''. destruct (eqDec n m) as [E|E].
+                { subst. rewrite bindSame, bindSame. apply equalRefl. }
+                { rewrite bindDiff, bindDiff.
+                    { apply H. simpl. apply remove_still; assumption. }
+                    { assumption. }
+                    { assumption. }}}
+Qed.
+
+Lemma evalEnvEqual : forall (e e':Env) (p:Formula),
+    envEqual e e' -> eval e p <-> eval e' p.
+Proof.
+    intros e e' p H. apply relevance. intros n H'. apply H.
+Qed.
+
+Lemma evalNotInFree : forall (e:Env) (n:nat) (x:set) (p:Formula),
+    ~In n (Fr p) -> eval (bind e n x) p <-> eval e p.
+Proof.
+    intros e n x p H. apply relevance. intros m H'. 
+    destruct (eqDec n m) as [E|E].
+    - subst. apply H in H'. contradiction.
+    - rewrite bindDiff. 
+        + apply equalRefl.
+        + assumption.
+Qed.
