coq/Logic/Lang1/Replacement.v
@@ -1,0 +1,19 @@
+Require Import List.
+
+Require Import Logic.Axiom.LEM.
+
+Require Import Logic.Set.Set.
+Require Import Logic.Set.Elem.
+Require Import Logic.Set.Incl.
+Require Import Logic.Set.Equal.
+Require Import Logic.Set.Compatible.
+
+Require Import Logic.Lang1.Syntax.
+Require Import Logic.Lang1.Semantics.
+Require Import Logic.Lang1.Relevance.
+Require Import Logic.Lang1.Environment.
+
+Definition replacementF (P:Formula) (n m p q:nat) : Formula :=
+    (Imp 
+        (Elem n n) (* TODO *)
+        (All n (Exi m (All p (Iff (Elem p m) (Exi q (And (Elem q n) P))))))).
