coq/Logic/Lang1/Semantics.v
@@ -1,0 +1,195 @@
+Import Nat.
+Require Import List.
+Require Import PeanoNat.
+
+Require Import Logic.Axiom.LEM.
+Require Import Logic.Nat.Fresh.
+
+Require Import Logic.Set.Set.
+Require Import Logic.Set.Incl.
+Require Import Logic.Set.Elem.
+Require Import Logic.Set.Equal.
+Require Import Logic.Set.Empty.
+Require Import Logic.Set.ElemIncl.
+Require Import Logic.Set.Foundation.
+
+Require Import Logic.Lang1.Valid.
+Require Import Logic.Lang1.Syntax.
+Require Import Logic.Lang1.Environment.
+
+Fixpoint eval (e:Env) (p:Formula) : Prop :=
+    match p with
+    | Bot           => False
+    | Elem n m      => (e n) :: (e m)
+    | Imp p1 p2     => eval e p1 -> eval e p2
+    | All n p1      => forall (x:set), eval (bind e n x) p1
+    end.
+
+(* Given an environement e, a formula p and a variable n, we can define a       *)
+(* predicate P: set -> Prop by defining P x as the proposition obtained by      *)
+(* evaluating the formula p in an environment where n is bound to x.            *)
+Definition eval1 (e:Env) (p:Formula) (n:nat) (x:set) : Prop :=
+    eval (bind e n x) p.
+
+(* Given an environement e, a formula p and two variables n m, we can define a  *)
+(* two variables predicate P: set -> set -> Prop by defining P x y as the pro-  *)
+(* position obtained by evaluating the formula p in an environment where n is   *)
+(* bound to x and m is bound to y. This predicate makes sense if n <> m.        *)
+Definition eval2 (e:Env) (p:Formula) (n m:nat) (x y:set) : Prop :=
+    eval (bind (bind e n x) m y) p.
+
+Lemma evalBot : forall (e:Env), eval e Bot <-> False.
+Proof. intros e. unfold eval. split; intros H; assumption. Qed.
+
+Lemma evalElem : forall (e:Env) (n m:nat), 
+    eval e (Elem n m) <-> (e n) :: (e m).
+Proof. intros e n m. unfold eval. split; intros H; assumption. Qed.
+
+Lemma evalImp : forall (e:Env) (p q:Formula),
+    eval e (Imp p q) <-> (eval e p -> eval e q).
+Proof.
+    intros e p q. unfold eval. fold (eval e p). fold (eval e q).
+    split; intros H; assumption.
+Qed.
+
+Lemma evalAll : forall (e:Env) (p:Formula) (n:nat),
+    eval e (All n p) <-> forall (x:set), eval (bind e n x) p.
+Proof.
+    intros e p n. unfold eval. split; intros H; assumption.
+Qed.
+
+Lemma evalNot : forall (e:Env) (p:Formula), 
+    eval e (Not p) <-> ~ eval e p.
+Proof. 
+    intros e p. unfold Not, eval. fold (eval e p).
+    split; intros H; assumption.
+Qed.
+
+Lemma evalOr : LEM -> forall (e:Env) (p q:Formula), 
+    eval e (Or p q) <-> eval e p \/ eval e q.
+Proof.
+    intros L e p q. unfold Or, eval. simpl. 
+    apply LEMOr. assumption.
+Qed.
+
+Lemma evalAnd : LEM -> forall (e:Env) (p q:Formula),
+    eval e (And p q) <-> eval e p /\ eval e q.
+Proof.
+    intros L e p q. unfold And, eval. simpl. 
+    apply LEMAnd. assumption.
+Qed.
+
+Lemma evalExi : LEM -> forall (e:Env) (p:Formula) (n:nat),
+    eval e (Exi n p) <-> exists (x:set), eval (bind e n x) p.
+Proof.
+    intros L e p n. unfold Exi, eval, bind. simpl. 
+    apply LEMExist. assumption.
+Qed.
+
+Lemma evalIff : LEM -> forall (e:Env) (p q:Formula),
+    eval e (Iff p q) <-> (eval e p <-> eval e q).
+Proof.
+    intros L e p q. unfold Iff. apply evalAnd. assumption.
+Qed.
+
+Lemma evalSub : LEM -> forall (e:Env) (n m:nat), 
+    eval e (Sub n m) <-> (e n) <= (e m).
+Proof.
+    intros L e n m. unfold Sub. rewrite elemIncl. 
+    rewrite evalAll. simpl. split; intros H z.
+    - remember (H z) as H' eqn:E. clear E.
+      rewrite bindSame in H'.
+      rewrite bindDiff in H'.
+      rewrite bindDiff in H'.
+        + assumption.
+        + apply freshNot_m. 
+        + apply freshNot_n.
+    - rewrite bindSame.
+      rewrite bindDiff.
+      rewrite bindDiff.
+        + apply H.
+        + apply freshNot_m.
+        + apply freshNot_n.
+Qed.
+
+Lemma evalEqu : LEM -> forall (e:Env) (n m:nat),
+    eval e (Equ n m) <-> (e n) == (e m).
+Proof.
+    intros L e n m. unfold Equ, equal. 
+    rewrite evalAnd, evalAll, evalAll. split; intros [H1 H2].
+    - split; intros z.
+        + remember (H1 z) as H1' eqn:E. clear E. 
+          rewrite evalIff in H1'.
+          rewrite evalElem in H1'.
+          rewrite evalElem in H1'.
+          rewrite bindSame in H1'.
+          rewrite bindDiff in H1'.
+          rewrite bindDiff in H1'.
+            { assumption. }
+            { apply freshNot_m. }
+            { apply freshNot_n. }
+            { assumption. }
+        + remember (H2 z) as H2' eqn:E. clear E. 
+          rewrite evalIff in H2'.
+          rewrite evalElem in H2'.
+          rewrite evalElem in H2'.
+          rewrite bindSame in H2'.
+          rewrite bindDiff in H2'.
+          rewrite bindDiff in H2'.
+            { assumption. }
+            { apply freshNot_m. }
+            { apply freshNot_n. }
+            { assumption. }
+    - split; intros z; 
+      rewrite evalIff, evalElem, evalElem, bindSame, bindDiff, bindDiff.
+        + apply H1.
+        + apply freshNot_m.
+        + apply freshNot_n.
+        + assumption.
+        + apply H2.
+        + apply freshNot_m.
+        + apply freshNot_n.
+        + assumption.
+    - assumption.
+Qed.
+
+Lemma evalEmpty : forall (e:Env) (n:nat),
+    eval e (Empty n) <-> (e n) == Nil. 
+Proof.
+    intros e n. unfold Empty. rewrite evalAll. split; intros H. 
+    - apply emptyUnique. intros x. remember (H x) as H' eqn:E. clear E. clear H.
+      rewrite evalNot in H'. rewrite evalElem in H'.
+      rewrite bindSame in H'. rewrite bindDiff in H'.
+        + assumption.
+        + apply freshNot_n.
+    - intro x. rewrite evalNot, evalElem, bindSame, bindDiff.
+      rewrite emptyIsNil in H. rewrite H.
+        + apply emptyCharac.
+        + apply freshNot_n.
+Qed.
+
+Lemma evalMin : LEM -> forall (e:Env) (n m:nat),
+    eval e (Min n m) <-> minimal (e n) (e m).
+Proof.
+    intros L e n m. unfold Min. rewrite evalAnd, evalElem, evalNot, evalExi.
+    unfold minimal. split; intros [H1 H2].
+    - split.
+        + assumption.
+        + intros [y H]. apply H2. exists y. rewrite evalAnd, evalElem, evalElem.
+          rewrite bindSame, bindDiff, bindDiff.
+            { assumption. }
+            { apply freshNot_n. }
+            { apply freshNot_m. }
+            { assumption. }
+    - split.
+        + assumption.
+        + intros [y H]. apply H2. exists y. rewrite evalAnd in H.
+          rewrite evalElem in H. rewrite evalElem in H. rewrite bindSame in H.
+          rewrite bindDiff in H. rewrite bindDiff in H.
+            { assumption. }
+            { apply freshNot_n. }
+            { apply freshNot_m. }
+            { assumption. }
+    - assumption.
+    - assumption.
+Qed.
