coq/Logic/Lang1/Specification.v
@@ -1,0 +1,153 @@
+Require Import List.  
+Require Import Logic.Axiom.LEM.
+Require Import Logic.List.Replace.
+
+Require Import Logic.Set.Set.
+Require Import Logic.Set.Elem.
+Require Import Logic.Set.Incl.
+Require Import Logic.Set.Equal.
+Require Import Logic.Set.Compatible.
+
+Require Import Logic.Lang1.Free.
+Require Import Logic.Lang1.Apply.
+Require Import Logic.Lang1.Valid.
+Require Import Logic.Lang1.Syntax.
+Require Import Logic.Lang1.Semantics.
+Require Import Logic.Lang1.Relevance.
+Require Import Logic.Lang1.Environment.
+
+(* Theorem schema of specification expressed in set theory abstract syntax.     *)
+(* The formulation is parameterized with respect to a formula P, hence this is  *)
+(* not a single theorem, but rather a 'theorem schema'. This formulation is     *)
+(* correct provided the variables n m p are distinct and m is not free in P.    *)
+Definition specificationF (P:Formula) (n m p:nat) : Formula :=
+    All n (Exi m (All p (Iff (Elem p m) (And (Elem p n) P)))). 
+
+(* Evaluating specificationF applied to a formula P in any environment 'yields' *)
+(* the theorem specificationDec' applied to the corresponding predicate.        *)
+Lemma evalSpecificationF : LEM -> forall (e:Env) (P: Formula) (n m p:nat),
+    m <> n ->
+    p <> n ->
+    p <> m ->
+    ~In m (Fr P) ->
+    eval e (specificationF P n m p)
+        <->
+    forall (x:set), exists (y:set), forall (z:set),
+        z :: y <-> z :: x /\ (eval2 e P n p x z).
+Proof.
+    intros L e P n m p Hmn Hpn Hpm NF. unfold specificationF. rewrite evalAll.
+    split; intros H x. 
+    - remember (H x) as H' eqn:E. clear E H. rewrite evalExi in H'.
+      destruct H' as [y H]. exists y. rewrite evalAll in H. intros z.
+      remember (H z) as H' eqn:E. clear E H. rewrite evalIff in H'.
+      rewrite evalElem in H'. rewrite evalAnd in H'. rewrite evalElem in H'.
+      rewrite bindSame in H'. rewrite bindDiff in H'. rewrite bindSame in H'.
+      rewrite bindDiff in H'. rewrite bindDiff in H'. rewrite bindSame in H'.
+      unfold eval2. destruct H' as [H1 H2]. split.
+        + rewrite <- (evalNotInFree (bind (bind e n x) p z)).
+            { rewrite (evalEnvEqual _ (bind (bind (bind e n x) m y) p z)). 
+                { assumption. }
+                { apply bindPermute. 
+                  intros Hmp. apply Hpm. symmetry. assumption. }}
+            { assumption. }
+        + intros [H3 H4]. apply H2. split.
+            { assumption. }
+            { rewrite (evalEnvEqual _ (bind (bind (bind e n x) p z) m y)).
+                { rewrite evalNotInFree; assumption. }
+                { apply bindPermute. assumption. }}
+        + assumption.
+        + assumption.
+        + assumption.
+        + assumption.
+        + assumption.
+        + assumption.
+    - rewrite evalExi. remember (H x) as H' eqn:E. clear E H.
+      destruct H' as [y H]. exists y. rewrite evalAll. intros z.
+      rewrite evalIff, evalElem, evalAnd, evalElem, bindSame.
+      rewrite bindDiff, bindSame, bindDiff, bindDiff, bindSame. 
+      remember (H z) as H' eqn:E. clear E H. unfold eval2 in H'. split.
+        + destruct H' as [H1 _]. intros H'.
+          remember (H1 H') as H eqn:E. clear E H1 H'. 
+          destruct H as [H1 H2]. split.
+            { assumption. }
+            { rewrite (evalEnvEqual _ (bind (bind (bind e n x) p z) m y)).
+                { rewrite evalNotInFree; assumption. }
+                { apply bindPermute. assumption. }}
+        + destruct H' as [_ H]. intros [H1 H2]. apply H. split.
+            { assumption. }
+            { rewrite (evalEnvEqual _ (bind (bind (bind e n x) p z) m y)) in H2.
+                { rewrite evalNotInFree in H2; assumption. }
+                { apply bindPermute. assumption. }}
+        + assumption.
+        + assumption.
+        + assumption.
+        + assumption.
+        + assumption.
+        + assumption.
+Qed.
+
+
+(* Theorem schema of specification where we explicitely 'apply' P at the        *)
+(* variables n and  p with 'apply2 P n p'.                                      *)
+Definition specificationF' (P:Formula) (n m p:nat) : Formula :=
+    All n (Exi m (All p (Iff (Elem p m) (And (Elem p n) (apply2 P n p))))). 
+
+(* Checking that the only difference between these statements is the apply2.    *)
+Local Lemma specificationLink_ : forall (P:Formula) (n m p:nat),
+    specificationF' P n m p = specificationF (apply2 P n p) n m p.
+Proof.
+    intros P n m p. reflexivity.
+Qed.
+
+Local Lemma specificationCarryOver_ : forall (p q: set -> set -> Prop),
+    (forall (x y:set), p x y <-> q x y) ->
+        (forall (x:set), exists (y:set), forall (z:set),
+            z :: y <-> z :: x /\ p x z)
+    <-> (forall (x:set), exists (y:set), forall (z:set),
+            z :: y <-> z :: x /\ q x z).
+Proof.
+    intros p q H1. split; intros H2 x; destruct (H2 x) as [y H3]; exists y;
+    intros z; destruct (H3 z) as [H4 H5]; split.
+    - intros H6. destruct (H4 H6) as [H7 H8]. split.
+        + assumption.
+        + apply H1. assumption.
+    - intros [H6 H7]. apply H5. split.
+        + assumption.
+        + apply H1. assumption.
+    - intros H6. destruct (H4 H6) as [H7 H8]. split.
+        + assumption.
+        + apply H1. assumption.
+    - intros [H6 H7]. apply H5. split.
+        + assumption.
+        + apply H1. assumption.
+Qed.
+
+(*
+(* Evaluating specificationF' applied to a formula P in any environment.        *)
+Lemma evalSpecificationF' : LEM -> forall (e:Env) (P: Formula) (n m p:nat),
+    m <> n ->
+    p <> n ->
+    p <> m ->
+    ~In m (Fr P) ->
+    ~In n (Fr P) ->
+    ~In p (Fr P) ->
+    Valid (replace2 0 1 n p) P ->
+    eval e (specificationF' P n m p)
+        <->
+    forall (x:set), exists (y:set), forall (z:set),
+        z :: y <-> z :: x /\ (eval2 e P 0 1 x z).
+Proof.
+    intros L e P n m p H1 H2 H3 H4 H5 H6 H7. rewrite specificationLink_. 
+    rewrite evalSpecificationF. apply specificationCarryOver_.
+    intros x y. apply evalApply2.
+    - assumption.
+    - assumption.
+    - assumption.
+    - intros H8. subst. apply H2. reflexivity.
+    - assumption.
+    - assumption.
+    - assumption.
+    - assumption.
+    -
+Show.
+*)
