coq/Logic/Lang1/Syntax.v
@@ -1,0 +1,44 @@
+Require Import Logic.Nat.Fresh.
+
+(* Abstract syntax for core language of types (propositions): Lang1.            *)
+(* There is no possibility of writing terms (proofs) in this language.          *)
+Inductive Formula : Type :=
+| Bot  : Formula
+| Elem : nat -> nat -> Formula
+| Imp  : Formula -> Formula -> Formula
+| All  : nat -> Formula -> Formula
+.
+
+(* Variable substitution mapping.                                               *)
+Fixpoint fmap (f:nat -> nat) (p:Formula) : Formula :=
+    match p with
+    | Bot       => Bot
+    | Elem x y  => Elem (f x) (f y)
+    | Imp p q   => Imp (fmap f p) (fmap f q)
+    | All x p   => All (f x) (fmap f p)
+    end.
+
+Definition Not (p:Formula)          :Formula := Imp p Bot.
+Definition Or  (p q:Formula)        :Formula := Imp (Not p) q.
+Definition And (p q:Formula)        :Formula := Not (Or (Not p) (Not q)).
+Definition Exi  (n:nat) (p:Formula) :Formula := Not (All n (Not p)).
+Definition Iff (p q:Formula)        :Formula := And (Imp p q) (Imp q p).
+
+Definition Sub (n m:nat) : Formula := 
+    let x := fresh n m in
+        All x (Imp (Elem x n) (Elem x m)).
+
+Definition Equ (n m:nat) : Formula := 
+    let x := fresh n m in And
+        (All x (Iff (Elem x n) (Elem x m)))
+        (All x (Iff (Elem n x) (Elem m x))).
+
+Definition Empty (n:nat) : Formula := 
+    let x := fresh n n in
+        All x (Not (Elem x n)).
+
+(* Predicate expressing the 'minimality' of a set n in a set m                  *)
+Definition Min (n m:nat) : Formula :=
+    let x := fresh n m in And
+        (Elem n m)
+        (Not (Exi x (And (Elem x m) (Elem x n)))).
