coq/Logic/Lang1/Union.v
@@ -1,0 +1,105 @@
+Require Import Logic.Axiom.LEM.
+
+Require Import Logic.Set.Set.
+Require Import Logic.Set.Elem.
+Require Import Logic.Set.Equal.
+
+Require Import Logic.Lang1.Syntax.
+Require Import Logic.Lang1.Semantics.
+Require Import Logic.Lang1.Environment.
+
+
+(* Theorem 'unionAxiom' expressed in set theory abstract syntax.                *)
+(* This formulation is correct provided the variables n m p q are distinct.     *)
+
+Definition unionAxiomF (n m p q:nat) : Formula :=
+    All n (Exi m (All p (Iff (Elem p m) (Exi q (And (Elem p q) (Elem q n)))))).
+
+
+(* Evaluating unionAxiomF in any environment 'yields' the theorem unionAxiom.   *)
+Lemma evalUnionAxiomF : LEM -> forall (e:Env) (n m p q:nat),
+    m <> n ->
+    p <> n ->
+    p <> m ->
+    q <> n ->
+    q <> m ->
+    q <> p ->
+    eval e (unionAxiomF n m p q)
+        <->
+    forall (x:set), exists (y:set), forall (z:set),
+        z :: y <-> exists (u:set), z :: u /\ u :: x. 
+Proof.
+    intros L e n m p q Hmn Hpn Hpm Hqn Hqm Hqp.
+    unfold unionAxiomF. rewrite evalAll. split; intros H x.
+    - remember (H x) as H' eqn:E. clear E. clear H. rewrite evalExi in H'.
+      destruct H' as [y H]. rewrite evalAll in H. exists y. intros z. 
+      remember (H z) as H' eqn:E. clear E. clear H. rewrite evalIff in H'.
+      remember (bind e n x) as e1 eqn:E1. remember (bind e1 m y) as e2 eqn:E2.
+      rewrite evalElem in H'. rewrite evalExi in H'. rewrite bindSame in H'.
+      rewrite bindDiff in H'. destruct H' as [H1 H2]. split; intros H0.
+        + rewrite E2 in H1. rewrite bindSame in H1.
+          remember (H1 H0) as H3 eqn:E. clear E. clear H1.
+          destruct H3 as [u H3]. exists u. rewrite evalAnd in H3.
+          rewrite evalElem in H3. rewrite evalElem in H3.
+          rewrite <- E2 in H3. remember (bind e2 p z) as e3 eqn:E3.
+          rewrite bindSame in H3. rewrite bindDiff in H3. rewrite bindDiff in H3.
+          rewrite E3 in H3. rewrite bindSame in H3. rewrite bindDiff in H3.
+          rewrite E2 in H3. rewrite bindDiff in H3. rewrite E1 in H3.
+          rewrite bindSame in H3.
+            { assumption. }
+            { assumption. }
+            { assumption. }
+            { assumption. }
+            { assumption. }
+            { assumption. }
+
+        + rewrite E2 in H2. rewrite bindSame in H2. apply H2.
+          destruct H0 as [u H3]. exists u. rewrite evalAnd, evalElem, evalElem.
+          rewrite <- E2. remember (bind e2 p z) as e3 eqn:E3.
+          rewrite bindSame, bindDiff, bindDiff, E3, bindSame, bindDiff, E2.
+          rewrite bindDiff, E1, bindSame.
+            { assumption. }
+            { assumption. }
+            { assumption. }
+            { assumption. }
+            { assumption. }
+            { assumption. }
+        + assumption.
+        + assumption.
+        + assumption.
+        + assumption.
+    - remember (H x) as H' eqn:E. clear E. clear H. destruct H' as [y H].
+      rewrite evalExi. exists y. rewrite evalAll. intros z.
+      rewrite evalIff, evalElem, evalExi.
+      remember (bind e n x) as e1 eqn:E1. remember (bind e1 m y) as e2 eqn:E2.
+      rewrite bindSame, bindDiff, E2, bindSame. split; intros H'.
+        + destruct (H z) as [H1 H2]. destruct (H1 H') as [u H3]. exists u.
+          rewrite evalAnd, evalElem, evalElem, <- E2.
+          remember (bind e2 p z) as e3 eqn:E3.
+          rewrite bindSame, bindDiff, E3, bindSame, bindDiff, bindDiff, E2.
+          rewrite bindDiff, E1, bindSame.
+            { assumption. }
+            { assumption. }
+            { assumption. }
+            { assumption. }
+            { assumption. }
+            { assumption. }
+        + destruct (H z) as [H1 H2]. apply H2. destruct H' as [u H3]. exists u.
+          rewrite evalAnd in H3. rewrite evalElem in H3. rewrite evalElem in H3.
+          rewrite <- E2 in H3. remember (bind e2 p z) as e3 eqn:E3.
+          rewrite bindSame in H3. rewrite bindDiff in H3. rewrite bindDiff in H3.
+          rewrite E3 in H3. rewrite bindSame in H3. rewrite bindDiff in H3.
+          rewrite E2 in H3. rewrite bindDiff in H3. rewrite E1 in H3.
+          rewrite bindSame in H3.
+            { assumption. }
+            { assumption. }
+            { assumption. }
+            { assumption. }
+            { assumption. }
+            { assumption. }
+        + assumption.
+        + assumption.
+        + assumption.
+        + assumption.
+Qed.
+
