coq/Logic/Nat/Eq.v
@@ -1,8 +1,14 @@
+Require Import Peano_dec.
+
+Require Import Logic.Class.Eq.
+
 Lemma not_eq_s_n : forall (n:nat), ~ S n = n.
 Proof.
     induction n as [|n IH]; intros H.
     - inversion H.
     - injection H. intros H'. apply IH. assumption.
 Qed.
+
+Instance EqNat : Eq nat := { eqDec := eq_nat_dec }.
 
 
