coq/Logic/Set/Functional.v
@@ -1,0 +1,5 @@
+Require Import Logic.Set.Set.
+Require Import Logic.Set.Equal.
+
+Definition functional (p:set -> set -> Prop) : Prop :=
+    forall (x y y':set), p x y -> p x y' -> y == y'.
