coq/Logic/Set/Normal/InListOf.v
@@ -1,0 +1,5 @@
+Require Import List.
+
+Require Import Logic.Set.Set.
+
+Definition inListOf (x xs:set) : Prop := In x (toList xs).
