coq/Logic/Set/Normal/Map.v
@@ -1,0 +1,20 @@
+Require List.
+
+Require Import Logic.Set.Set.
+Require Import Logic.Set.Normal.InListOf.
+
+Definition map (f:set -> set) (x:set) : set :=
+    fromList (List.map f (toList x)).
+
+Lemma mapCons : forall (f:set -> set) (x xs:set),
+    map f (Cons x xs) = Cons (f x) (map f xs).
+Proof.
+    intros f x xs. unfold map. simpl. reflexivity.
+Qed.
+
+Lemma inListOfMapIff : forall (y xs:set) (f:set -> set),
+    inListOf y (map f xs) <-> (exists (x:set), f x = y /\ inListOf x xs).
+Proof.
+    intros y xs f. unfold inListOf, map. rewrite toListFromList.
+    apply List.in_map_iff.
+Qed.
