coq/Logic/Set/Normal/Ord.v
@@ -1,0 +1,14 @@
+Require Import Logic.Set.Set.
+
+Require Import Logic.Class.Ord.
+
+Require Import Logic.Set.Normal.Leq.
+
+Instance ordSet : Ord set :=
+    { leq      := leq
+    ; leqDec   := leqDec
+    ; leqRefl  := leqRefl
+    ; leqTrans := leqTrans
+    ; leqAsym  := leqASym
+    ; leqTotal := leqTotal
+    }. 
