coq/Logic/Set/Replacement.v
@@ -1,0 +1,109 @@
+Require Import List.
+
+Require Import Logic.Axiom.LEM.
+Require Import Logic.List.Filter.
+
+Require Import Logic.Set.Set.
+Require Import Logic.Set.Incl.
+Require Import Logic.Set.Elem.
+Require Import Logic.Set.Equal.
+Require Import Logic.Set.ToList.
+Require Import Logic.Set.Functional.
+Require Import Logic.Set.Compatible.
+Require Import Logic.Set.Extensionality.
+
+Require Import Logic.Set.Normal.Normal.
+
+(* Axiom schema of replacement assuming LEM for our Coq meta-logic.             *)
+Theorem replacementLEM : forall (p:set -> set -> Prop),
+    LEM ->
+    compatible2 p ->
+    functional p  -> 
+    forall (x:set),
+        exists (y:set), forall (z:set),
+            z :: y <-> exists (u:set), u :: x /\ p u z.
+Proof.
+    intros p L C F x. 
+    remember (toList x) as xs eqn:H1.
+    remember (fun x y => p x y /\ Normal y) as q eqn:Q.
+    assert (forall (x:set) (y y':set), q x y -> q x y' -> y = y') as H2.
+    { rewrite Q. intros u y y' [H3 H4] [H5 H6]. apply normalEqualSame.
+        { assumption. }
+        { assumption. }
+        { apply (F u); assumption. } }
+    assert (exists (ys:list set), forall (y:set), 
+        In y ys <-> exists (u:set), In u xs /\ q u y) as H3.
+    { apply filterReplace; assumption. }
+    destruct H3 as [ys H3]. exists (fromList ys). intros z. split; intros H4.
+    - rewrite toListElem, toListFromList in H4. destruct H4 as [z' [H4 [H5 H6]]].
+      apply H3 in H4. rewrite Q in H4. destruct H4 as [u [H7 [H8 H9]]].    
+      exists u. split.
+        + apply toListElem. exists u. split.
+            { rewrite <- H1. assumption. }
+            { split; apply inclRefl. }
+        + apply (C u u z' z).
+            { apply equalRefl. }
+            { apply doubleIncl. split; assumption. }
+            { assumption. }
+    - apply toListElem. rewrite toListFromList. remember (normal z) as z' eqn:Z.
+      exists z'. destruct H4 as [u [H4 H5]]. apply toListElem in H4. 
+      destruct H4 as [u' [H4 [H6 H7]]]. split.
+        + apply H3. exists u'. split.
+            { rewrite H1. assumption. }
+            { rewrite Q. split.
+                { apply (C u u' z z').
+                    { apply doubleIncl. split; assumption. }
+                    { rewrite Z. apply equalSym, normalEqual. }
+                    { assumption. }}
+                { rewrite Z. apply normalNormal. }}
+        + apply doubleIncl. rewrite Z. apply equalSym, normalEqual. 
+Qed.
+
+(* Again, this is simply to demonstrate explicit dependency in x in not needed. *)
+Corollary replacementLEM_ : forall (p:set -> set -> set -> Prop),
+    LEM ->
+    compatible3 p ->
+    forall (x:set),
+    functional (p x)  -> 
+        exists (y:set), forall (z:set),
+            z :: y <-> exists (u:set), u :: x /\ p x u z.
+Proof.
+    intros p L C x F. apply replacementLEM. 
+    - assumption.
+    - apply Comp3Comp2. assumption.
+    - assumption.
+Qed.
+
+
+(* A proof of the axiom schema of specification based on replacement.           *)
+Theorem specificationLEM : forall (p:set -> Prop), 
+    LEM ->
+    compatible p -> 
+    forall (x:set), exists (y:set), forall (z:set), 
+        z :: y <-> z :: x /\ p z.
+Proof.
+    intros p L C. remember (fun x y => p x /\ (x == y)) as q eqn:Q.
+    assert (compatible2 q) as Cq.
+        { unfold compatible2. rewrite Q. intros x x' y y' H1 H2 [H3 H4]. split.
+            { apply (C x x'); assumption. }
+            { apply equalTrans with x.
+                { apply equalSym. assumption. }
+                { apply equalTrans with y; assumption. }}}
+    assert (functional q) as Fq.
+        { unfold functional. rewrite Q. intros x y y' [H1 H2] [H3 H4].
+          apply equalTrans with x.
+            { apply equalSym. assumption. }
+            { assumption. }}
+    intros x. remember (replacementLEM q L Cq Fq x) as R eqn:E. clear E. 
+    destruct R as [y R]. exists y. intros z. destruct (R z) as [H1 H2]. 
+    rewrite Q in H1. split; intros H.
+    -  apply H1 in H. clear H1 H2.
+      destruct H as [u [H1 [H2 H3]]]. split.
+        + apply elemCompatL with u; assumption.
+        + apply (C u z); assumption.
+    - apply H2. exists z. destruct H as [H3 H4]. split.
+        + assumption.
+        + rewrite Q. split.
+            { assumption. }
+            { apply equalRefl. }
+Qed.
