coq/Logic/Set/Specification.v
@@ -1,0 +1,116 @@
+Require Import List.
+
+Require Import Logic.Axiom.LEM.
+Require Import Logic.Axiom.Decidable.
+
+Require Import Logic.List.Filter.
+
+Require Import Logic.Set.Set.
+Require Import Logic.Set.Incl.
+Require Import Logic.Set.Elem.
+Require Import Logic.Set.Equal.
+Require Import Logic.Set.ToList.
+Require Import Logic.Set.Compatible.
+Require Import Logic.Set.Extensionality.
+
+(* The axiom schema of specification is implied by that of replacement.         *)
+
+(* Given a set x and a decidable predicate p (which may depend on x), returns   *)
+(* the set of all elements y of x for which p y is true. There is no need to    *)
+(* consider p a two variable predicate in order to make the possible dependency *)
+(* in the set x explicit. This single variable formalism will do just as well.  *)
+Definition comp (x:set)(p:set -> Prop)(q:Dec p) : set :=
+    fromList (filter q (toList x)).
+
+(* The predicate needs to be decidable and compatible.                          *)
+Lemma compCharac : forall (x:set) (p:set -> Prop) (q:Dec p), 
+    compatible p ->
+    forall (z:set), z :: comp x p q <-> z :: x /\ p z.
+Proof.
+    intros x p q C z. unfold comp. split; intros H.
+    - apply toListElem in H. destruct H as [y [H1 [H2 H3]]].
+      rewrite toListFromList in H1. rewrite <- filterEquiv in H1.
+      destruct H1 as [H0 H1]. split.
+        + apply toListElem. exists y. split.
+            { assumption. }
+            { split; assumption. }
+        + unfold compatible in C. apply C with y.
+            { apply doubleIncl. split; assumption. }
+            { assumption. }
+    - destruct H as [H0 H1]. apply toListElem. apply toListElem in H0.
+      destruct H0 as [y [H0 [H2 H3]]]. exists y. rewrite toListFromList. split.
+        + apply filterEquiv. split.
+            { assumption. }
+            { unfold compatible in C. apply C with z.
+                { apply doubleIncl. split; assumption. }
+                { assumption. }}
+        + split; assumption.
+Qed.
+
+(* Axiom schema of specification true in our model for decidable predicates.    *)
+Theorem specificationDec : forall (p:set -> Prop), 
+    Dec p ->
+    compatible p ->
+    forall (x:set), exists (y:set), forall (z:set), 
+        z :: y <-> z :: x /\ p z.
+Proof.
+    intros p D C x. exists (comp x p D). apply compCharac. assumption.
+Qed.
+
+(* This is to emphasize that the predicate p above may depend on x. It is an    *)
+(* immediate consequence of the main result so not very useful. It only serves  *)
+(* to show there is no need to make dependency in x explicit in main result.    *)
+Corollary specificationDec_ : forall (p:set -> set -> Prop), 
+    Dec2 p          ->
+    compatible2 p   ->
+    forall (x:set), exists (y:set), forall (z:set), 
+        z :: y <-> z :: x /\ p x z.  (* explicit dependency in x *)
+Proof.
+    intros p D C x. apply specificationDec.
+    - apply Dec2Dec. assumption.
+    - apply Comp2Comp. assumption. 
+Qed.
+
+(* Axiom schema of specification for weaker assumption of weak decidability.    *)
+(* Again, there is no need to make possible dependency in x explicit in p.      *)
+Theorem specificationDec' : forall (p:set -> Prop), 
+    Dec' p ->
+    compatible p -> 
+    forall (x:set), exists (y:set), forall (z:set), 
+        z :: y <-> z :: x /\ p z.
+Proof.
+    intros p D C x. 
+    remember (filterDec' set p D (toList x)) as H eqn:E. clear E.
+    destruct H as [ys H]. exists (fromList ys). intros z. split; intros H'.
+    - apply toListElem in H'. destruct H' as [z' H']. 
+      rewrite toListFromList in H'. destruct H' as [H0 [H1 H2]]. 
+      remember (H z') as H3 eqn:E. clear E H. destruct H3 as [H3 H4]. 
+      apply H4 in H0. destruct H0 as [H0 H5]. split.
+        + apply toListElem. exists z'. split.
+            {  assumption. }
+            { split; assumption. }
+        + unfold compatible in C. apply C with z'.
+            { apply doubleIncl. split; assumption. }
+            { assumption. }
+    - destruct H' as [H0 H1]. rewrite toListElem in H0.
+      destruct H0 as [z' [H0 [H2 H3]]]. apply toListElem. exists z'.
+      rewrite toListFromList. split.
+        + apply H. split.
+            { assumption. }
+            { unfold compatible in C. apply C with z.
+                { apply doubleIncl. split; assumption. }
+                { assumption. }}
+        + split; assumption.
+Qed.
+
+(* Again, this is simply to demonstrate explicit dependency in x in not needed. *)
+Corollary specificationDec'_ : forall (p:set -> set -> Prop), 
+    Dec2' p ->
+    compatible2 p -> 
+    forall (x:set), exists (y:set), forall (z:set), 
+        z :: y <-> z :: x /\ p x z.
+Proof.
+    intros p D C x. apply specificationDec'.
+    - apply Dec2Dec'. assumption.
+    - apply Comp2Comp. assumption.
+Qed.
