coq/set/Utils/Include.v
@@ -1,8 +1,0 @@
-Require Import List.
-
-Lemma inclNil : forall (a:Type) (xs:list a), incl xs nil -> xs = nil.
-Proof.
-    intros a. destruct xs as [|x xs]; intros H.
-    - reflexivity.
-    - exfalso. destruct (H x). left. reflexivity.
-Qed.
