coq/Logic/clean.sh
@@ -4,5 +4,7 @@ DIR=/home/john/Prog/coq/Logic
 cd ${DIR}
 
 make clean > /dev/null
+rm -rf *.vo *.glob .*.aux .shake
+
 
 
