coq/Logic/deps.sh
@@ -1,0 +1,24 @@
+#!/bin/sh
+
+# Creates dependendy files needed for inclusion in Makefile
+
+DIR=$(pwd)
+
+# Temporary files are created on the /tmp directory to avoid race
+# condition with the 'grep -r'
+
+# Processing 'Require Import'
+grep 'Require Import Logic\.' -r | cat - > /tmp/deps
+sed -i 's/\.v\:Require Import Logic\./.vo:/g' /tmp/deps
+sed -i 's/\.vo\:\([[:alnum:]]*\)\.\([[:alnum:]]*\)\.\([[:alnum:]]*\)\./.vo : \1\/\2\/\3.vo/g' /tmp/deps
+sed -i 's/\.vo\:\([[:alnum:]]*\)\.\([[:alnum:]]*\)\./.vo : \1\/\2.vo/g' /tmp/deps
+
+# Ssimilar process for dependencies without 'Import', just 'Require'
+grep 'Require Logic\.' -r | cat - > /tmp/deps_
+sed -i 's/\.v\:Require Logic\./.vo:/g' /tmp/deps_
+sed -i 's/\.vo\:\([[:alnum:]]*\)\.\([[:alnum:]]*\)\.\([[:alnum:]]*\)\./.vo : \1\/\2\/\3.vo/g' /tmp/deps_
+sed -i 's/\.vo\:\([[:alnum:]]*\)\.\([[:alnum:]]*\)\./.vo : \1\/\2.vo/g' /tmp/deps_
+
+cat /tmp/deps_ >> /tmp/deps
+mv /tmp/deps ${DIR}/deps
+rm -f /tmp/deps /tmp/deps_
