coq/set/Utils/Eq.v
@@ -1,4 +1,0 @@
-Class Eq (a:Type) :=
-    { eqDec : forall (x y:a), { x = y }   + { ~ x = y }
-    }.
-
